test.dfy
@@ -1,0 +1,24 @@
+method Max(a: int, b: int) returns (res: int)
+  // Fill in the 'ensures' clauses here to prove the two points above!
+  ensures res >= a && res >= b
+  ensures res == a || res == b
+{
+  if a > b {
+    res := a;
+  } else {
+    res := b;
+  }
+}
+
+method Main() {
+  var a := 10;
+  var b := 20;
+  var m := Max(a, b);
+  
+  // Because of your 'ensures' clauses, Dafny knows this is true:
+  assert m == 20; 
+  assert m >= a;
+  assert m >= b;
+  
+  print m;
+}
